MLIR/Semantics/Fitree.lean
@@ -248,3 +248,13 @@ elab "simp_itree" : tactic => do
     StateT.bind, StateT.pure, StateT.lift,
     OptionT.bind, OptionT.pure, OptionT.mk, OptionT.lift,
     bind, pure, cast_eq, Eq.mpr])
+
+elab "dsimp_itree" : tactic => do
+  -- TODO: Also handle .lemmaNames, not just unfolding!
+  let lemmas := (← SimpItreeExtension.getTheorems).toUnfold.fold
+    (init := #[]) (fun acc n => acc.push (toSimpLemma n))
+  evalTactic $ ← `(tactic|dsimp [$(⟨lemmas.reverse⟩),*,
+    Member.inject,
+    StateT.bind, StateT.pure, StateT.lift,
+    OptionT.bind, OptionT.pure, OptionT.mk, OptionT.lift,
+    bind, pure, cast_eq, Eq.mpr])
